src/smtencoding/FStarC.SMTEncoding.Term.fsti
@@ -269,6 +269,7 @@ val mkForall:  Range.range -> (list (list pat) & fvs & term) -> term
 val mkForall': Range.range -> (list (list pat) & option int & fvs & term)  -> term
 val mkForall'': Range.range -> (list (list pat) & option int & list sort & term) -> term
 val mkExists: Range.range -> (list (list pat) & fvs & term) -> term
+val mkForallFlat:  (fvs & term) -> term
 val mkLet: (list term & term) -> Range.range -> term
 val mkLet': (list (fv & term) & term) -> Range.range -> term
 
